<?xml version="1.0"?>


<!DOCTYPE rdf:RDF [
    <!ENTITY owl "http://www.w3.org/2002/07/owl#" >
    <!ENTITY obo "http://purl.obolibrary.org/obo/" >
    <!ENTITY dc "http://purl.org/dc/elements/1.1/" >
    <!ENTITY xsd "http://www.w3.org/2001/XMLSchema#" >
    <!ENTITY snap "http://www.ifomis.org/bfo/1.1/snap#" >
    <!ENTITY span "http://www.ifomis.org/bfo/1.1/span#" >
    <!ENTITY rdfs "http://www.w3.org/2000/01/rdf-schema#" >
    <!ENTITY rdf "http://www.w3.org/1999/02/22-rdf-syntax-ns#" >
]>


<rdf:RDF xmlns="&obo;MF#"
     xml:base="&obo;MF"
     xmlns:dc="http://purl.org/dc/elements/1.1/"
     xmlns:obo="http://purl.obolibrary.org/obo/"
     xmlns:rdfs="http://www.w3.org/2000/01/rdf-schema#"
     xmlns:snap="http://www.ifomis.org/bfo/1.1/snap#"
     xmlns:owl="http://www.w3.org/2002/07/owl#"
     xmlns:xsd="http://www.w3.org/2001/XMLSchema#"
     xmlns:rdf="http://www.w3.org/1999/02/22-rdf-syntax-ns#"
     xmlns:span="http://www.ifomis.org/bfo/1.1/span#">
    <owl:Ontology rdf:about="&obo;MF">
        <dc:contributor>Mark Jensen</dc:contributor>
        <dc:contributor>Werner Ceusters</dc:contributor>
        <dc:title>The Ontology of Mental Functioning (MF) was first described in the publication available at http://www.jbiomedsem.com/content/1/1/10 entitled &#39;Foundations for a realist ontology of mental disease&#39; (Barry Smith and Werner Ceusters). </dc:title>
        <rdfs:comment>This OWL version of the MF ontology was created by Janna Hastings</rdfs:comment>
        <dc:contributor>Barry Smith</dc:contributor>
        <dc:contributor>Janna Hastings</dc:contributor>
        <dc:description>The Mental Functioning Ontology is an overarching ontology for all aspects of mental functioning, founded on the Basic Formal Ontology (BFO) and related to the Ontology for General Medical Science (OGMS).</dc:description>
        <owl:imports rdf:resource="&obo;iao.owl"/>
        <owl:imports rdf:resource="http://www.ifomis.org/bfo/1.1"/>
    </owl:Ontology>
    


    <!-- 
    ///////////////////////////////////////////////////////////////////////////////////////
    //
    // Annotation properties
    //
    ///////////////////////////////////////////////////////////////////////////////////////
     -->

    <owl:AnnotationProperty rdf:about="&dc;contributor"/>
    <owl:AnnotationProperty rdf:about="&rdfs;label"/>
    <owl:AnnotationProperty rdf:about="&rdfs;comment"/>
    <owl:AnnotationProperty rdf:about="&dc;title"/>
    


    <!-- 
    ///////////////////////////////////////////////////////////////////////////////////////
    //
    // Datatypes
    //
    ///////////////////////////////////////////////////////////////////////////////////////
     -->

    


    <!-- 
    ///////////////////////////////////////////////////////////////////////////////////////
    //
    // Object Properties
    //
    ///////////////////////////////////////////////////////////////////////////////////////
     -->

    


    <!-- http://purl.obolibrary.org/obo/MF#hasAgent -->

    <owl:ObjectProperty rdf:about="&obo;MF#hasAgent"/>
    


    <!-- http://purl.obolibrary.org/obo/MF#hasPart -->

    <owl:ObjectProperty rdf:about="&obo;MF#hasPart"/>
    


    <!-- http://purl.obolibrary.org/obo/MF#hasParticipant -->

    <owl:ObjectProperty rdf:about="&obo;MF#hasParticipant"/>
    


    <!-- http://purl.obolibrary.org/obo/MF#inhererOf -->

    <owl:ObjectProperty rdf:about="&obo;MF#inhererOf"/>
    


    <!-- http://purl.obolibrary.org/obo/MF#inheresIn -->

    <owl:ObjectProperty rdf:about="&obo;MF#inheresIn"/>
    


    <!-- http://purl.obolibrary.org/obo/MF#isAbout -->

    <owl:ObjectProperty rdf:about="&obo;MF#isAbout"/>
    


    <!-- http://purl.obolibrary.org/obo/MF#manifestationOf -->

    <owl:ObjectProperty rdf:about="&obo;MF#manifestationOf"/>
    


    <!-- http://purl.obolibrary.org/obo/MF#partOf -->

    <owl:ObjectProperty rdf:about="&obo;MF#partOf"/>
    


    <!-- http://purl.obolibrary.org/obo/MF#participantOf -->

    <owl:ObjectProperty rdf:about="&obo;MF#participantOf"/>
    


    <!-- http://purl.obolibrary.org/obo/MF#realizationOf -->

    <owl:ObjectProperty rdf:about="&obo;MF#realizationOf"/>
    


    <!-- http://purl.obolibrary.org/obo/MF#specificallyDependsOn -->

    <owl:ObjectProperty rdf:about="&obo;MF#specificallyDependsOn"/>
    


    <!-- 
    ///////////////////////////////////////////////////////////////////////////////////////
    //
    // Classes
    //
    ///////////////////////////////////////////////////////////////////////////////////////
     -->

    


    <!-- http://purl.obolibrary.org/obo/MF_0000000 -->

    <owl:Class rdf:about="&obo;MF_0000000">
        <rdfs:label rdf:datatype="&xsd;string">Mental Functioning Related Anatomical Structure</rdfs:label>
        <rdfs:subClassOf rdf:resource="&obo;MF_0000007"/>
        <rdfs:subClassOf>
            <owl:Restriction>
                <owl:onProperty rdf:resource="&obo;MF#inhererOf"/>
                <owl:someValuesFrom rdf:resource="&obo;MF_0000001"/>
            </owl:Restriction>
        </rdfs:subClassOf>
        <obo:IAO_0000115>ANATOMICAL STRUCTURE in which there inheres the DISPOSITION to be the agent
of a MENTAL PROCESS.
Source:
http://www.jbiomedsem.com/content/1/1/10</obo:IAO_0000115>
    </owl:Class>
    


    <!-- http://purl.obolibrary.org/obo/MF_0000001 -->

    <owl:Class rdf:about="&obo;MF_0000001">
        <rdfs:label rdf:datatype="&xsd;string">Disposition to be agentOf Mental Process</rdfs:label>
        <rdfs:subClassOf rdf:resource="&snap;Disposition"/>
        <rdfs:subClassOf>
            <owl:Restriction>
                <owl:onProperty rdf:resource="&obo;MF#inheresIn"/>
                <owl:someValuesFrom rdf:resource="&obo;MF_0000000"/>
            </owl:Restriction>
        </rdfs:subClassOf>
    </owl:Class>
    


    <!-- http://purl.obolibrary.org/obo/MF_0000002 -->

    <owl:Class rdf:about="&obo;MF_0000002">
        <rdfs:label rdf:datatype="&xsd;string">Disposition to lead to Pathological Mental Processes</rdfs:label>
        <rdfs:subClassOf rdf:resource="&obo;MF_0000006"/>
    </owl:Class>
    


    <!-- http://purl.obolibrary.org/obo/MF_0000003 -->

    <owl:Class rdf:about="&obo;MF_0000003">
        <rdfs:label rdf:datatype="&xsd;string">Behavior Inducing State</rdfs:label>
        <rdfs:subClassOf rdf:resource="&obo;MF_0000009"/>
        <rdfs:subClassOf>
            <owl:Restriction>
                <owl:onProperty rdf:resource="&obo;MF#participantOf"/>
                <owl:someValuesFrom rdf:resource="&obo;MF_0000022"/>
            </owl:Restriction>
        </rdfs:subClassOf>
        <rdfs:subClassOf>
            <owl:Restriction>
                <owl:onProperty rdf:resource="&obo;MF#inheresIn"/>
                <owl:someValuesFrom rdf:resource="&obo;MF_0000000"/>
            </owl:Restriction>
        </rdfs:subClassOf>
        <obo:IAO_0000115>BODILY QUALITY inhering in a MENTAL
FUNCTIONING RELATED ANATOMICAL STRUCTURE which leads to BEHAVIOR of some
specific sort.
Source:
http://www.jbiomedsem.com/content/1/1/10</obo:IAO_0000115>
    </owl:Class>
    


    <!-- http://purl.obolibrary.org/obo/MF_0000004 -->

    <owl:Class rdf:about="&obo;MF_0000004">
        <rdfs:label rdf:datatype="&xsd;string">Mental Disorder</rdfs:label>
        <rdfs:subClassOf rdf:resource="&obo;MF_0000010"/>
        <rdfs:subClassOf>
            <owl:Restriction>
                <owl:onProperty rdf:resource="&obo;MF#partOf"/>
                <owl:someValuesFrom rdf:resource="&obo;MF_0000000"/>
            </owl:Restriction>
        </rdfs:subClassOf>
        <obo:IAO_0000115>DISORDER in a MENTAL FUNCTIONING
RELATED ANATOMICAL STRUCTURE.
Source:
http://www.jbiomedsem.com/content/1/1/10</obo:IAO_0000115>
    </owl:Class>
    


    <!-- http://purl.obolibrary.org/obo/MF_0000005 -->

    <owl:Class rdf:about="&obo;MF_0000005">
        <rdfs:label rdf:datatype="&xsd;string">Mental Disease</rdfs:label>
        <rdfs:subClassOf rdf:resource="&obo;MF_0000002"/>
        <obo:IAO_0000115>a DISEASE which is a DISPOSITION to undergo
PATHOLOGICAL MENTAL PROCESSES.
Source:
http://www.jbiomedsem.com/content/1/1/10</obo:IAO_0000115>
    </owl:Class>
    


    <!-- http://purl.obolibrary.org/obo/MF_0000006 -->

    <owl:Class rdf:about="&obo;MF_0000006">
        <rdfs:label rdf:datatype="&xsd;string">Disposition to lead to Pathological Processes</rdfs:label>
        <rdfs:subClassOf rdf:resource="&snap;Disposition"/>
    </owl:Class>
    


    <!-- http://purl.obolibrary.org/obo/MF_0000007 -->

    <owl:Class rdf:about="&obo;MF_0000007">
        <rdfs:label rdf:datatype="&xsd;string">Anatomical Structure</rdfs:label>
        <rdfs:subClassOf rdf:resource="&snap;IndependentContinuant"/>
        <rdfs:subClassOf>
            <owl:Restriction>
                <owl:onProperty rdf:resource="&obo;MF#partOf"/>
                <owl:someValuesFrom rdf:resource="&obo;MF_0000015"/>
            </owl:Restriction>
        </rdfs:subClassOf>
    </owl:Class>
    


    <!-- http://purl.obolibrary.org/obo/MF_0000009 -->

    <owl:Class rdf:about="&obo;MF_0000009">
        <rdfs:label rdf:datatype="&xsd;string">Bodily Quality</rdfs:label>
        <rdfs:subClassOf rdf:resource="&snap;Quality"/>
        <rdfs:subClassOf>
            <owl:Restriction>
                <owl:onProperty rdf:resource="&obo;MF#inheresIn"/>
                <owl:someValuesFrom rdf:resource="&obo;MF_0000012"/>
            </owl:Restriction>
        </rdfs:subClassOf>
        <obo:IAO_0000115>QUALITY inhering in a BODILY COMPONENT.
Source:
http://www.jbiomedsem.com/content/1/1/10.</obo:IAO_0000115>
        <rdfs:comment>(from OGMS)</rdfs:comment>
    </owl:Class>
    


    <!-- http://purl.obolibrary.org/obo/MF_0000010 -->

    <owl:Class rdf:about="&obo;MF_0000010">
        <rdfs:label rdf:datatype="&xsd;string">Disorder</rdfs:label>
        <rdfs:subClassOf rdf:resource="&obo;MF_0000012"/>
        <obo:IAO_0000115>A combination of BODILY COMPONENTS of or in
an ORGANISM that is clinically abnormal.
Source:
http://www.jbiomedsem.com/content/1/1/10</obo:IAO_0000115>
        <rdfs:comment>(from OGMS)</rdfs:comment>
    </owl:Class>
    


    <!-- http://purl.obolibrary.org/obo/MF_0000011 -->

    <owl:Class rdf:about="&obo;MF_0000011">
        <rdfs:label rdf:datatype="&xsd;string">Disease</rdfs:label>
        <rdfs:subClassOf rdf:resource="&obo;MF_0000006"/>
        <obo:IAO_0000115>a DISPOSITION (i) to undergo PATHOLOGICAL
PROCESSES that (ii) exists in an ORGANISM
because of one or more DISORDERS in that
ORGANISM.
Source:
http://www.jbiomedsem.com/content/1/1/10</obo:IAO_0000115>
        <rdfs:comment>(from OGMS)</rdfs:comment>
    </owl:Class>
    


    <!-- http://purl.obolibrary.org/obo/MF_0000012 -->

    <owl:Class rdf:about="&obo;MF_0000012">
        <rdfs:label rdf:datatype="&xsd;string">Bodily Component</rdfs:label>
        <rdfs:subClassOf rdf:resource="&obo;MF_0000014"/>
        <obo:IAO_0000115>MATERIAL OBJECT within or on the surface of an
ORGANISM, including ANATOMICAL
STRUCTURES, body flora, pathogens, toxins, and
their combinations, potentially including also the
organism as a whole.
Source: http://www.jbiomedsem.com/content/1/1/10.</obo:IAO_0000115>
        <rdfs:comment>(from OGMS)</rdfs:comment>
    </owl:Class>
    


    <!-- http://purl.obolibrary.org/obo/MF_0000014 -->

    <owl:Class rdf:about="&obo;MF_0000014">
        <rdfs:label rdf:datatype="&xsd;string">Material Object</rdfs:label>
        <rdfs:subClassOf rdf:resource="&snap;IndependentContinuant"/>
    </owl:Class>
    


    <!-- http://purl.obolibrary.org/obo/MF_0000015 -->

    <owl:Class rdf:about="&obo;MF_0000015">
        <rdfs:label rdf:datatype="&xsd;string">Organism</rdfs:label>
        <rdfs:subClassOf rdf:resource="&obo;MF_0000014"/>
    </owl:Class>
    


    <!-- http://purl.obolibrary.org/obo/MF_0000016 -->

    <owl:Class rdf:about="&obo;MF_0000016">
        <rdfs:label rdf:datatype="&xsd;string">Human Being</rdfs:label>
        <rdfs:subClassOf rdf:resource="&obo;MF_0000015"/>
    </owl:Class>
    


    <!-- http://purl.obolibrary.org/obo/MF_0000020 -->

    <owl:Class rdf:about="&obo;MF_0000020">
        <rdfs:label rdf:datatype="&xsd;string">Mental Process</rdfs:label>
        <rdfs:subClassOf rdf:resource="&obo;MF_0000026"/>
        <rdfs:subClassOf>
            <owl:Restriction>
                <owl:onProperty rdf:resource="&obo;MF#realizationOf"/>
                <owl:someValuesFrom rdf:resource="&obo;MF_0000001"/>
            </owl:Restriction>
        </rdfs:subClassOf>
        <rdfs:subClassOf>
            <owl:Restriction>
                <owl:onProperty rdf:resource="&obo;MF#hasParticipant"/>
                <owl:someValuesFrom rdf:resource="&obo;MF_0000003"/>
            </owl:Restriction>
        </rdfs:subClassOf>
        <obo:IAO_0000115>BODILY PROCESS which brings into being,
sustains or modifies a COGNITIVE REPRESENTATION or a BEHAVIOR INDUCING
STATE.
Source:
http://www.jbiomedsem.com/content/1/1/10</obo:IAO_0000115>
    </owl:Class>
    


    <!-- http://purl.obolibrary.org/obo/MF_0000021 -->

    <owl:Class rdf:about="&obo;MF_0000021">
        <rdfs:label rdf:datatype="&xsd;string">Interpersonal Process</rdfs:label>
        <rdfs:subClassOf rdf:resource="&span;Process"/>
        <rdfs:subClassOf>
            <owl:Restriction>
                <owl:onProperty rdf:resource="&obo;MF#hasParticipant"/>
                <owl:onClass rdf:resource="&obo;MF_0000016"/>
                <owl:minQualifiedCardinality rdf:datatype="&xsd;nonNegativeInteger">2</owl:minQualifiedCardinality>
            </owl:Restriction>
        </rdfs:subClassOf>
        <obo:IAO_0000115>PROCESS in which at least two HUMAN
BEINGS are agents.
Source:
http://www.jbiomedsem.com/content/1/1/10</obo:IAO_0000115>
    </owl:Class>
    


    <!-- http://purl.obolibrary.org/obo/MF_0000022 -->

    <owl:Class rdf:about="&obo;MF_0000022">
        <rdfs:label rdf:datatype="&xsd;string">Behavior</rdfs:label>
        <rdfs:subClassOf rdf:resource="&span;Process"/>
        <rdfs:subClassOf>
            <owl:Restriction>
                <owl:onProperty rdf:resource="&obo;MF#hasAgent"/>
                <owl:someValuesFrom rdf:resource="&obo;MF_0000015"/>
            </owl:Restriction>
        </rdfs:subClassOf>
        <obo:IAO_0000115>a PROCESS having PROCESSES as parts in which an
ORGANISM participates as agent in response to external or internal stimuli and
following some pattern which is dependent upon some combination of that
ORGANISM’s internal state and external conditions. (Derived from the Gene
Ontology).
Source:
http://www.jbiomedsem.com/content/1/1/10</obo:IAO_0000115>
    </owl:Class>
    


    <!-- http://purl.obolibrary.org/obo/MF_0000023 -->

    <owl:Class rdf:about="&obo;MF_0000023">
        <rdfs:label rdf:datatype="&xsd;string">Interpersonal Behavior</rdfs:label>
        <rdfs:subClassOf rdf:resource="&obo;MF_0000022"/>
        <rdfs:subClassOf>
            <owl:Restriction>
                <owl:onProperty rdf:resource="&obo;MF#hasPart"/>
                <owl:someValuesFrom rdf:resource="&obo;MF_0000021"/>
            </owl:Restriction>
        </rdfs:subClassOf>
        <obo:IAO_0000115>BEHAVIOR having INTERPERSONAL
PROCESSES as parts, each involving the same instances of HUMAN BEING.
Source:
http://www.jbiomedsem.com/content/1/1/10</obo:IAO_0000115>
    </owl:Class>
    


    <!-- http://purl.obolibrary.org/obo/MF_0000024 -->

    <owl:Class rdf:about="&obo;MF_0000024">
        <rdfs:label rdf:datatype="&xsd;string">Pathological Mental Process</rdfs:label>
        <rdfs:subClassOf rdf:resource="&obo;MF_0000020"/>
        <rdfs:subClassOf>
            <owl:Restriction>
                <owl:onProperty rdf:resource="&obo;MF#manifestationOf"/>
                <owl:someValuesFrom rdf:resource="&obo;MF_0000004"/>
            </owl:Restriction>
        </rdfs:subClassOf>
        <obo:IAO_0000115>PATHOLOGICAL PROCESS
which is the manifestation of a MENTAL DISORDER.
Source:
http://www.jbiomedsem.com/content/1/1/10</obo:IAO_0000115>
    </owl:Class>
    


    <!-- http://purl.obolibrary.org/obo/MF_0000025 -->

    <owl:Class rdf:about="&obo;MF_0000025">
        <rdfs:label rdf:datatype="&xsd;string">Mental Disease Course</rdfs:label>
        <rdfs:subClassOf rdf:resource="&obo;MF_0000029"/>
        <rdfs:subClassOf>
            <owl:Restriction>
                <owl:onProperty rdf:resource="&obo;MF#hasPart"/>
                <owl:someValuesFrom rdf:resource="&obo;MF_0000024"/>
            </owl:Restriction>
        </rdfs:subClassOf>
        <obo:IAO_0000115>DISEASE COURSE of a MENTAL DISEASE.
Source:
http://www.jbiomedsem.com/content/1/1/10</obo:IAO_0000115>
    </owl:Class>
    


    <!-- http://purl.obolibrary.org/obo/MF_0000026 -->

    <owl:Class rdf:about="&obo;MF_0000026">
        <rdfs:label rdf:datatype="&xsd;string">Bodily Process</rdfs:label>
        <rdfs:subClassOf rdf:resource="&span;Process"/>
        <rdfs:subClassOf>
            <owl:Restriction>
                <owl:onProperty rdf:resource="&obo;MF#hasParticipant"/>
                <owl:someValuesFrom rdf:resource="&obo;MF_0000012"/>
            </owl:Restriction>
        </rdfs:subClassOf>
        <obo:IAO_0000115>PROCESS in which at least one BODILY
COMPONENT of an ORGANISM participates.
Source:
http://www.jbiomedsem.com/content/1/1/10
</obo:IAO_0000115>
        <rdfs:comment>(from OGMS)</rdfs:comment>
    </owl:Class>
    


    <!-- http://purl.obolibrary.org/obo/MF_0000028 -->

    <owl:Class rdf:about="&obo;MF_0000028">
        <rdfs:label rdf:datatype="&xsd;string">Pathological Process</rdfs:label>
        <rdfs:subClassOf rdf:resource="&obo;MF_0000026"/>
        <rdfs:subClassOf>
            <owl:Restriction>
                <owl:onProperty rdf:resource="&obo;MF#manifestationOf"/>
                <owl:someValuesFrom rdf:resource="&obo;MF_0000010"/>
            </owl:Restriction>
        </rdfs:subClassOf>
        <rdfs:comment>(from OGMS)</rdfs:comment>
        <obo:IAO_0000115>a BODILY PROCESS that is a manifestation of a
DISORDER.
Source:
http://www.jbiomedsem.com/content/1/1/10
</obo:IAO_0000115>
    </owl:Class>
    


    <!-- http://purl.obolibrary.org/obo/MF_0000029 -->

    <owl:Class rdf:about="&obo;MF_0000029">
        <rdfs:label rdf:datatype="&xsd;string">Disease Course</rdfs:label>
        <rdfs:subClassOf rdf:resource="&span;Process"/>
        <rdfs:subClassOf>
            <owl:Restriction>
                <owl:onProperty rdf:resource="&obo;MF#hasPart"/>
                <owl:someValuesFrom rdf:resource="&obo;MF_0000028"/>
            </owl:Restriction>
        </rdfs:subClassOf>
        <rdfs:comment>(from OGMS)</rdfs:comment>
        <obo:IAO_0000115>the totality of all PROCESSES through which a
given DISEASE instance is realized.
Source:
http://www.jbiomedsem.com/content/1/1/10

</obo:IAO_0000115>
    </owl:Class>
    


    <!-- http://purl.obolibrary.org/obo/MF_0000030 -->

    <owl:Class rdf:about="&obo;MF_0000030">
        <rdfs:label rdf:datatype="&xsd;string">Representation</rdfs:label>
        <rdfs:subClassOf rdf:resource="&snap;DependentContinuant"/>
        <obo:IAO_0000115>DEPENDENT CONTINUANT which is about a
portion of reality.
Source:
http://www.jbiomedsem.com/content/1/1/10</obo:IAO_0000115>
    </owl:Class>
    


    <!-- http://purl.obolibrary.org/obo/MF_0000031 -->

    <owl:Class rdf:about="&obo;MF_0000031">
        <rdfs:label rdf:datatype="&xsd;string">Cognitive Representation</rdfs:label>
        <rdfs:subClassOf rdf:resource="&obo;MF_0000030"/>
        <rdfs:subClassOf>
            <owl:Restriction>
                <owl:onProperty rdf:resource="&obo;MF#specificallyDependsOn"/>
                <owl:someValuesFrom rdf:resource="&obo;MF_0000007"/>
            </owl:Restriction>
        </rdfs:subClassOf>
        <obo:IAO_0000115>REPRESENTATION which
specifically depends on an ANATOMICAL STRUCTURE in the cognitive system of an
ORGANISM.</obo:IAO_0000115>
    </owl:Class>
    


    <!-- http://purl.obolibrary.org/obo/MF_0000032 -->

    <owl:Class rdf:about="&obo;MF_0000032">
        <rdfs:label rdf:datatype="&xsd;string">Observation</rdfs:label>
        <rdfs:subClassOf rdf:resource="&obo;MF_0000031"/>
        <rdfs:subClassOf>
            <owl:Restriction>
                <owl:onProperty rdf:resource="&obo;MF#isAbout"/>
                <owl:someValuesFrom rdf:resource="&obo;MF_0000009"/>
            </owl:Restriction>
        </rdfs:subClassOf>
        <rdfs:comment>(from OGMS)</rdfs:comment>
        <obo:IAO_0000115>COGNITIVE REPRESENTATION about a BODILY
FEATURE resulting from an act of perception.
Source:
http://www.jbiomedsem.com/content/1/1/10</obo:IAO_0000115>
    </owl:Class>
    


    <!-- http://purl.obolibrary.org/obo/MF_0000033 -->

    <owl:Class rdf:about="&obo;MF_0000033">
        <rdfs:label rdf:datatype="&xsd;string">Diagnosis</rdfs:label>
        <rdfs:subClassOf rdf:resource="&obo;MF_0000030"/>
        <rdfs:subClassOf>
            <owl:Restriction>
                <owl:onProperty rdf:resource="&obo;MF#isAbout"/>
                <owl:someValuesFrom rdf:resource="&obo;MF_0000011"/>
            </owl:Restriction>
        </rdfs:subClassOf>
        <obo:IAO_0000115>REPRESENTATION asserting the presence of an
instance of DISEASE in a given ORGANISM
resulting from an interpretive process that has as
input a CLINICAL PICTURE of that ORGANISM.
Source:
http://www.jbiomedsem.com/content/1/1/10</obo:IAO_0000115>
        <rdfs:comment>(from OGMS)</rdfs:comment>
    </owl:Class>
    


    <!-- http://purl.obolibrary.org/obo/MF_0000034 -->

    <owl:Class rdf:about="&obo;MF_0000034">
        <rdfs:label rdf:datatype="&xsd;string">Disease Picture</rdfs:label>
        <rdfs:subClassOf rdf:resource="&obo;MF_0000030"/>
        <rdfs:subClassOf>
            <owl:Restriction>
                <owl:onProperty rdf:resource="&obo;MF#isAbout"/>
                <owl:someValuesFrom rdf:resource="&obo;MF_0000042"/>
            </owl:Restriction>
        </rdfs:subClassOf>
        <obo:IAO_0000115>REPRESENTATION of a DISEASE PHENOTYPE
concretized in some information artifact.
Source:
http://www.jbiomedsem.com/content/1/1/10</obo:IAO_0000115>
    </owl:Class>
    


    <!-- http://purl.obolibrary.org/obo/MF_0000035 -->

    <owl:Class rdf:about="&obo;MF_0000035">
        <rdfs:label rdf:datatype="&xsd;string">Representational Unit</rdfs:label>
        <rdfs:subClassOf rdf:resource="&obo;MF_0000030"/>
        <obo:IAO_0000115>REPRESENTATION none of whose proper parts are themselves
representations. Source: http://www.jbiomedsem.com/content/1/1/10</obo:IAO_0000115>
    </owl:Class>
    


    <!-- http://purl.obolibrary.org/obo/MF_0000036 -->

    <owl:Class rdf:about="&obo;MF_0000036">
        <rdfs:label rdf:datatype="&xsd;string">Disease Picture Component</rdfs:label>
        <rdfs:subClassOf rdf:resource="&obo;MF_0000035"/>
        <rdfs:subClassOf>
            <owl:Restriction>
                <owl:onProperty rdf:resource="&obo;MF#isAbout"/>
                <owl:someValuesFrom rdf:resource="&obo;MF_0000009"/>
            </owl:Restriction>
        </rdfs:subClassOf>
        <rdfs:subClassOf>
            <owl:Restriction>
                <owl:onProperty rdf:resource="&obo;MF#partOf"/>
                <owl:someValuesFrom rdf:resource="&obo;MF_0000034"/>
            </owl:Restriction>
        </rdfs:subClassOf>
        <obo:IAO_0000115>REPRESENTATIONAL UNIT which
is a part of some DISEASE PICTURE and which either (1) represents (or is believed to
represent) a BODILY FEATURE that is believed to be manifested in the DISEASE
PHENOTYPE represented by the DISEASE PICTURE of which it is a component or (2)
expresses a negative finding. 
Source:
http://www.jbiomedsem.com/content/1/1/10</obo:IAO_0000115>
    </owl:Class>
    


    <!-- http://purl.obolibrary.org/obo/MF_0000037 -->

    <owl:Class rdf:about="&obo;MF_0000037">
        <rdfs:label rdf:datatype="&xsd;string">Clinical Picture</rdfs:label>
        <rdfs:subClassOf rdf:resource="&obo;MF_0000030"/>
        <rdfs:subClassOf>
            <owl:Restriction>
                <owl:onProperty rdf:resource="&obo;MF#isAbout"/>
                <owl:someValuesFrom rdf:resource="&obo;MF_0000043"/>
            </owl:Restriction>
        </rdfs:subClassOf>
        <obo:IAO_0000115>A CLINICAL PICTURE is a REPRESENTATION of a CLINICAL PHENOTYPE
that is inferred from the combination of laboratory,
image and clinical findings about a given
ORGANISM.
Source:
http://www.jbiomedsem.com/content/1/1/10</obo:IAO_0000115>
        <rdfs:comment>(from OGMS)</rdfs:comment>
    </owl:Class>
    


    <!-- http://purl.obolibrary.org/obo/MF_0000038 -->

    <owl:Class rdf:about="&obo;MF_0000038">
        <rdfs:label rdf:datatype="&xsd;string">Marker features</rdfs:label>
        <rdfs:subClassOf rdf:resource="&obo;MF_0000030"/>
        <rdfs:subClassOf>
            <owl:Restriction>
                <owl:onProperty rdf:resource="&obo;MF#hasPart"/>
                <owl:someValuesFrom rdf:resource="&obo;MF_0000036"/>
            </owl:Restriction>
        </rdfs:subClassOf>
        <obo:IAO_0000115>REPRESENTATION which is a collection of DISEASE PICTURE COMPONENTS which
are characteristic for DISEASE X (where ‘X’ serves as placeholder for some disease
name).
Source:
http://www.jbiomedsem.com/content/1/1/10</obo:IAO_0000115>
    </owl:Class>
    


    <!-- http://purl.obolibrary.org/obo/MF_0000039 -->

    <owl:Class rdf:about="&obo;MF_0000039">
        <rdfs:label rdf:datatype="&xsd;string">Affective Representation</rdfs:label>
        <rdfs:subClassOf rdf:resource="&obo;MF_0000031"/>
        <obo:IAO_0000115>COGNITIVE REPRESENTATION
sustained by an ORGANISM about its own emotions.
Source:
http://www.jbiomedsem.com/content/1/1/10</obo:IAO_0000115>
    </owl:Class>
    


    <!-- http://purl.obolibrary.org/obo/MF_0000040 -->

    <owl:Class rdf:about="&obo;MF_0000040">
        <rdfs:label rdf:datatype="&xsd;string">Diagnosis of Mental Disease</rdfs:label>
        <rdfs:subClassOf rdf:resource="&obo;MF_0000033"/>
        <obo:IAO_0000115>DIAGNOSIS asserting the
presence of an instance of MENTAL DISEASE in a given ORGANISM.
Source:
http://www.jbiomedsem.com/content/1/1/10</obo:IAO_0000115>
    </owl:Class>
    


    <!-- http://purl.obolibrary.org/obo/MF_0000041 -->

    <owl:Class rdf:about="&obo;MF_0000041">
        <rdfs:label rdf:datatype="&xsd;string">Manifestation of a Mental Disease</rdfs:label>
        <rdfs:subClassOf rdf:resource="&obo;MF_0000009"/>
        <rdfs:subClassOf>
            <owl:Restriction>
                <owl:onProperty rdf:resource="&obo;MF#realizationOf"/>
                <owl:someValuesFrom rdf:resource="&obo;MF_0000005"/>
            </owl:Restriction>
        </rdfs:subClassOf>
        <obo:IAO_0000115>a BODILY FEATURE of
an ORGANISM that is (a) a deviation from clinical normality that is the realization of
a MENTAL DISEASE and is (b) observable.
Source:
http://www.jbiomedsem.com/content/1/1/10</obo:IAO_0000115>
    </owl:Class>
    


    <!-- http://purl.obolibrary.org/obo/MF_0000042 -->

    <owl:Class rdf:about="&obo;MF_0000042">
        <rdfs:label rdf:datatype="&xsd;string">Disease Phenotype</rdfs:label>
        <rdfs:subClassOf rdf:resource="&obo;MF_0000043"/>
        <obo:IAO_0000115>a CLINICAL PHENOTYPE that is characteristic of a
single DISEASE.
Source:
http://www.jbiomedsem.com/content/1/1/10</obo:IAO_0000115>
        <rdfs:comment>(from OGMS)</rdfs:comment>
    </owl:Class>
    


    <!-- http://purl.obolibrary.org/obo/MF_0000043 -->

    <owl:Class rdf:about="&obo;MF_0000043">
        <rdfs:label rdf:datatype="&xsd;string">Clinical Phenotype</rdfs:label>
        <rdfs:subClassOf rdf:resource="&obo;MF_0000047"/>
        <obo:IAO_0000115>a clinically abnormal PHENOTYPE.
Source:
http://www.jbiomedsem.com/content/1/1/10
</obo:IAO_0000115>
        <rdfs:comment>(from OGMS)</rdfs:comment>
    </owl:Class>
    


    <!-- http://purl.obolibrary.org/obo/MF_0000047 -->

    <owl:Class rdf:about="&obo;MF_0000047">
        <rdfs:label rdf:datatype="&xsd;string">Phenotype</rdfs:label>
        <rdfs:subClassOf rdf:resource="&obo;MF_0000009"/>
        <rdfs:comment>(from OGMS)</rdfs:comment>
        <obo:IAO_0000115>a combination of one or more BODILY FEATURES
of an ORGANISM determined by the interaction of
its genetic make-up and environment.
Source:
http://www.jbiomedsem.com/content/1/1/10</obo:IAO_0000115>
    </owl:Class>
    


    <!-- http://www.ifomis.org/bfo/1.1/snap#Disposition -->

    <owl:Class rdf:about="&snap;Disposition"/>
    


    <!-- http://www.ifomis.org/bfo/1.1/snap#GenericallyDependentContinuant -->

    <owl:Class rdf:about="&snap;GenericallyDependentContinuant"/>
    


    <!-- http://www.ifomis.org/bfo/1.1/snap#IndependentContinuant -->

    <owl:Class rdf:about="&snap;IndependentContinuant"/>
    


    <!-- http://www.ifomis.org/bfo/1.1/snap#Quality -->

    <owl:Class rdf:about="&snap;Quality"/>
    


    <!-- http://www.ifomis.org/bfo/1.1/span#Process -->

    <owl:Class rdf:about="&span;Process"/>
</rdf:RDF>



<!-- Generated by the OWL API (version 3.2.3.1824) http://owlapi.sourceforge.net -->

